{
 "cells": [
  {
   "cell_type": "markdown",
   "metadata": {},
   "source": [
    "# 1 written: Understand word2vec\n",
    "\n",
    "**(a)** $$ - \\sum_w y_w \\log{\\hat{y}_w} = - \\sum_{w \\neq o} 0 \\times \\log{\\hat{y}_w} - 1 \\times \\log{\\hat{y}_o} = -\\log{\\hat{y}_o}$$"
   ]
  },
  {
   "cell_type": "markdown",
   "metadata": {},
   "source": [
    "**(b)**\n",
    "Change the matrix formulation in J to scala.\n",
    "\n",
    "$$\n",
    "J = (\\ln{\\sum_w e^{\\sum_i (u_w)_i (v_c)_i}}) - \\sum_{i} (u_o)_i (v_c)_i \n",
    "$$\n",
    "$$\n",
    "\\frac{\\partial{J}}{\\partial{(v_c)_a}} = \\frac{\\sum_b (u_b)_a e^{\\sum_i (u_b)_i (v_c)_i}}{\\sum_w e^{\\sum_i (u_w)_i (v_c)_i}} - (u_o)_a\n",
    "$$\n",
    "\n",
    "Given that \n",
    "$$\n",
    "\\hat{y}_b = \\frac{e^{\\sum_i (u_b)_i (v_c)_i}}{\\sum_w e^{\\sum_i (u_w)_i (v_c)_i}}\n",
    "$$\n",
    "and \n",
    "$$\n",
    "(u_b)_a = U_{ab}\n",
    "$$\n",
    "We have\n",
    "$$\n",
    "\\frac{\\partial{J}}{\\partial{(v_c)_a}} = \\sum_b U_{ab} \\hat{y}_b - (u_o)_a\n",
    "$$\n",
    "\n",
    "\n",
    "Range a from 1 to n(the length of the vector) and we get\n",
    "\n",
    "$$\n",
    "\\frac{\\partial{J}}{\\partial{(v_c)}} = U\\hat{y}-u_o\n",
    "$$\n",
    "Besides, \n",
    "$$\n",
    "u_o = Uy\n",
    "$$\n",
    "Therefore,\n",
    "$$\n",
    "\\frac{\\partial{J}}{\\partial{(v_c)}} = U(\\hat{y}-y)\n",
    "$$"
   ]
  },
  {
   "cell_type": "markdown",
   "metadata": {},
   "source": [
    "**(b)** Another mothod: backprop\n",
    "\n",
    "define\n",
    "$$\n",
    "x = U^T v_c \n",
    "$$\n",
    "x is a vector, then, \n",
    "$$\n",
    "\\hat{y}_i = \\frac{e^{x_i}}{\\sum_w  e^{x_w}}\n",
    "$$\n",
    "$$\n",
    "J = \\ln{\\sum_w  e^{x_w}} - x_o\n",
    "$$\n",
    "$$\n",
    "\\frac{\\partial J}{\\partial x_i} = \\frac{e^{x_i}}{\\sum_w  e^{x_w}} - \\delta_{oi}\n",
    "$$\n",
    "Range 1 from 1 to n(the length of the vector) and we get\n",
    "$$\n",
    "\\frac{\\partial J}{\\partial x} = \\hat{y} - y\n",
    "$$\n",
    "use backprop\n",
    "$$\n",
    "\\frac{\\partial J}{\\partial (v_c)_a} = \\sum_j \\frac{\\partial J}{\\partial x_j} \\frac{\\partial x_j}{\\partial (v_c)_a} \n",
    "$$\n",
    "Let's first look at $\\frac{\\partial x_j}{\\partial (v_c)_a} $\n",
    "$$\n",
    "\\frac{\\partial x_j}{\\partial (v_c)_a} = \\frac{\\partial \\sum_k U^T_{jk}(v_c)_k}{\\partial (v_c)_a}\n",
    "= \\frac{\\partial U^T_{ja}(v_c)_a}{\\partial (v_c)_a} = U^T_{ja} = U_{aj}\n",
    "$$\n",
    "$$\n",
    "\\frac{\\partial J}{\\partial (v_c)_a} =\\sum_j U_{aj} (\\hat{y_j} - y_j)\n",
    "$$\n",
    "$$\n",
    "\\frac{\\partial J}{\\partial (v_c)} = U(\\hat{y}-y)\n",
    "$$"
   ]
  },
  {
   "cell_type": "markdown",
   "metadata": {},
   "source": [
    "**(c)**\n",
    "\n",
    "still use back prop\n",
    "$$\n",
    "\\frac{\\partial J}{\\partial x} = \\hat{y} - y\n",
    "$$\n",
    "$$\n",
    "\\frac{\\partial J}{\\partial U_{ab}} = \\sum_j \\frac{\\partial J}{\\partial x_j} \\frac{\\partial x_j}{\\partial U_ab} \n",
    "$$\n",
    "$$\n",
    "\\frac{\\partial x_j}{\\partial U_ab} = \\frac{\\partial \\sum_k U^T_{jk}(v_c)_k}{\\partial U_{ab}}=\\delta_{jb} (v_c)_a\n",
    "$$\n",
    "$$\n",
    "\\frac{\\partial J}{\\partial U_{ab}} = \\sum_j \\frac{\\partial J}{\\partial x_j} \\delta_{jb} (v_c)_a = \\frac{\\partial J}{\\partial x_b} (v_c)_a = (v_c)_a(\\hat{y}_b - y_b)\n",
    "$$\n",
    "$$\n",
    "\\frac{\\partial J}{\\partial U} = v_c (\\hat{y} - y)^T\n",
    "$$\n",
    "when $w=o$\n",
    "$$\n",
    "\\frac{\\partial J}{\\partial U} = v_c (\\hat{y}_w - 1)\n",
    "$$\n",
    "when $w \\neq o$\n",
    "$$\n",
    "\\frac{\\partial J}{\\partial U} = v_c \\hat{y}_w \n",
    "$$"
   ]
  },
  {
   "cell_type": "markdown",
   "metadata": {},
   "source": [
    "**(d)** change the problem to compute the derivative of $\\sigma(x^Ty)$ (x and y are column vector) with respect to x and y respectively.\n",
    "\n",
    "backprop\n",
    "\n",
    "$$\n",
    "\\frac{\\partial \\sigma(a)}{\\partial a} = \\sigma(a)(1-\\sigma(a))\n",
    "$$\n",
    "where a is scala $x^Ty$.\n",
    "\n",
    "$$\n",
    "\\frac{\\partial x^Ty}{\\partial x} = y\n",
    "$$\n",
    "\n",
    "$$\n",
    "\\frac{\\partial x^Ty}{\\partial y} = x\n",
    "$$\n",
    "\n",
    "$$\n",
    "\\frac{\\partial \\sigma(x^Ty)}{\\partial x} = \\sigma(x^Ty)(1-\\sigma(x^Ty))y\n",
    "$$\n",
    "\n",
    "$$\n",
    "\\frac{\\partial \\sigma(x^Ty)}{\\partial y} = \\sigma(x^Ty)(1-\\sigma(x^Ty))x\n",
    "$$\n",
    "\n",
    "furthermore, we can get\n",
    "$$\n",
    "\\frac{\\partial \\ln{\\sigma(x^Ty)}}{\\partial x} = (1-\\sigma(x^Ty))y\n",
    "$$\n",
    "\n",
    "$$\n",
    "\\frac{\\partial \\ln{\\sigma(x^Ty)}}{\\partial y} = (1-\\sigma(x^Ty))x\n",
    "$$\n"
   ]
  },
  {
   "cell_type": "markdown",
   "metadata": {},
   "source": [
    "**(e)** Using the conclusion in (d), we can get the answer directly.\n",
    "\n",
    "$$\n",
    "\\frac{\\partial J}{\\partial u_o} = -(1 - \\sigma(u_o^T v_c))v_c\n",
    "$$\n",
    "$$\n",
    "\\frac{\\partial J}{\\partial u_k} = (1 - \\sigma(-u_k^T v_c))v_c\n",
    "$$\n",
    "$$\n",
    "\\frac{\\partial J}{\\partial v_c} = -(1 - \\sigma(u_o^T v_c))u_o  + \\sum_{k=1}^K(1 - \\sigma(-u_k^T v_c))u_k\n",
    "$$\n",
    "\n",
    "\n",
    "***Reason***\n",
    "\n",
    "This function only concern about K negative outside words while the naive-softmax function required all words to be considered as outside words."
   ]
  },
  {
   "cell_type": "markdown",
   "metadata": {},
   "source": [
    "**(f)**\n",
    "\n",
    "(i) \n",
    "$$\n",
    "\\sum_{-m \\leq j \\leq m, j\\neq 0 } \\frac{\\partial J(v_c, w_{t+j}, U)}{\\partial U}\n",
    "$$\n",
    "(ii)\n",
    "$$\n",
    "\\sum_{-m \\leq j \\leq m, j\\neq 0 } \\frac{\\partial J(v_c, w_{t+j}, U)}{\\partial v_c}\n",
    "$$\n",
    "(iii)\n",
    "$$\n",
    "0\n",
    "$$"
   ]
  },
  {
   "cell_type": "code",
   "execution_count": null,
   "metadata": {},
   "outputs": [],
   "source": []
  }
 ],
 "metadata": {
  "kernelspec": {
   "display_name": "liu",
   "language": "python",
   "name": "liu"
  },
  "language_info": {
   "codemirror_mode": {
    "name": "ipython",
    "version": 3
   },
   "file_extension": ".py",
   "mimetype": "text/x-python",
   "name": "python",
   "nbconvert_exporter": "python",
   "pygments_lexer": "ipython3",
   "version": "3.7.2"
  }
 },
 "nbformat": 4,
 "nbformat_minor": 2
}
